refactor: pull up the call to bitblaster up as much as possible

LeanSAT/Reflect/BVExpr/BitBlast/Impl/Pred.lean
@@ -1,28 +1,55 @@
 import LeanSAT.Reflect.BVExpr.BitBlast.Impl.Eq
 import LeanSAT.Reflect.BVExpr.BitBlast.Impl.Ult
 import LeanSAT.Reflect.BVExpr.BitBlast.Impl.GetLsb
+import LeanSAT.Reflect.BVExpr.BitBlast.Impl.Expr
 
 namespace BVPred
 
 def bitblast (aig : AIG BVBit) (pred : BVPred) : AIG.Entrypoint BVBit :=
   match pred with
   | .bin lhs op rhs =>
+    let res := lhs.bitblast aig
+    let aig := res.aig
+    let lhsRefs := res.stream
+    let res := rhs.bitblast aig
+    let aig := res.aig
+    let rhsRefs := res.stream
+    let lhsRefs := lhsRefs.cast <| by
+      simp (config := { zetaDelta := true }) only
+      apply AIG.LawfulStreamOperator.le_size (f := BVExpr.bitblast)
     match op with
-    | .eq => mkEq aig ⟨lhs, rhs⟩
-    | .ult => mkUlt aig ⟨lhs, rhs⟩
-  | .getLsb expr idx => blastGetLsb aig ⟨expr, idx⟩
+    | .eq => mkEq aig ⟨lhsRefs, rhsRefs⟩
+    | .ult => mkUlt aig ⟨lhsRefs, rhsRefs⟩
+  | .getLsb expr idx =>
+    /-
+    Note: This blasts the entire rexpression up to `w` despite only needing it up to `idx`.
+    However the vast majority of operations are interested in all bits so the API is currently
+    not designed to support this use case.
+    -/
+    let res := expr.bitblast aig
+    let aig := res.aig
+    let refs := res.stream
+    blastGetLsb aig ⟨refs, idx⟩
 
 theorem bitblast_le_size (aig : AIG BVBit) (pred : BVPred)
     : aig.decls.size ≤ (bitblast aig pred).aig.decls.size := by
   cases pred with
   | bin lhs op rhs =>
-    cases op
-    all_goals
-      simp only [bitblast]
-      apply AIG.LawfulOperator.le_size
+    cases op with
+    | eq =>
+      simp [bitblast]
+      apply AIG.LawfulOperator.le_size_of_le_aig_size (f := mkEq)
+      apply AIG.LawfulStreamOperator.le_size_of_le_aig_size (f := BVExpr.bitblast)
+      apply AIG.LawfulStreamOperator.le_size (f := BVExpr.bitblast)
+    | ult =>
+      simp [bitblast]
+      apply AIG.LawfulOperator.le_size_of_le_aig_size (f := mkUlt)
+      apply AIG.LawfulStreamOperator.le_size_of_le_aig_size (f := BVExpr.bitblast)
+      apply AIG.LawfulStreamOperator.le_size (f := BVExpr.bitblast)
   | getLsb expr idx =>
     simp only [bitblast]
-    apply AIG.LawfulOperator.le_size
+    apply AIG.LawfulOperator.le_size_of_le_aig_size (f := blastGetLsb)
+    apply AIG.LawfulStreamOperator.le_size (f := BVExpr.bitblast)
 
 theorem bitblast_decl_eq (aig : AIG BVBit) (pred : BVPred) {h : idx < aig.decls.size} :
     have := bitblast_le_size aig pred
@@ -33,12 +60,29 @@ theorem bitblast_decl_eq (aig : AIG BVBit) (pred : BVPred) {h : idx < aig.decls.
     | eq =>
       simp only [bitblast]
       rw [AIG.LawfulOperator.decl_eq (f := mkEq)]
+      rw [AIG.LawfulStreamOperator.decl_eq (f := BVExpr.bitblast)]
+      rw [AIG.LawfulStreamOperator.decl_eq (f := BVExpr.bitblast)]
+      . apply AIG.LawfulStreamOperator.lt_size_of_lt_aig_size (f := BVExpr.bitblast)
+        assumption
+      . apply AIG.LawfulStreamOperator.lt_size_of_lt_aig_size (f := BVExpr.bitblast)
+        apply AIG.LawfulStreamOperator.le_size_of_le_aig_size (f := BVExpr.bitblast)
+        assumption
     | ult =>
       simp only [bitblast]
       rw [AIG.LawfulOperator.decl_eq (f := mkUlt)]
+      rw [AIG.LawfulStreamOperator.decl_eq (f := BVExpr.bitblast)]
+      rw [AIG.LawfulStreamOperator.decl_eq (f := BVExpr.bitblast)]
+      . apply AIG.LawfulStreamOperator.lt_size_of_lt_aig_size (f := BVExpr.bitblast)
+        assumption
+      . apply AIG.LawfulStreamOperator.lt_size_of_lt_aig_size (f := BVExpr.bitblast)
+        apply AIG.LawfulStreamOperator.le_size_of_le_aig_size (f := BVExpr.bitblast)
+        assumption
   | getLsb expr idx =>
     simp only [bitblast]
     rw [AIG.LawfulOperator.decl_eq (f := blastGetLsb)]
+    rw [AIG.LawfulStreamOperator.decl_eq (f := BVExpr.bitblast)]
+    apply AIG.LawfulStreamOperator.lt_size_of_lt_aig_size (f := BVExpr.bitblast)
+    assumption
 
 instance : AIG.LawfulOperator BVBit (fun _ => BVPred) bitblast where
   le_size := bitblast_le_size
