LeanSAT/Reflect/BVExpr/BitBlast/Impl/Ult.lean
@@ -1,21 +1,12 @@
-import LeanSAT.Reflect.BVExpr.BitBlast.Impl.Expr
 import LeanSAT.Reflect.BVExpr.BitBlast.Impl.Carry
+import LeanSAT.Reflect.BVExpr.BitBlast.Impl.Not
 
 namespace BVPred
 
-def mkUlt (aig : AIG BVBit) (pair : ExprPair) : AIG.Entrypoint BVBit :=
-  let res := pair.lhs.bitblast aig
-  let aig := res.aig
-  let lhsRefs := res.stream
-  let res := pair.rhs.bitblast aig
-  let aig := res.aig
-  let rhsRefs := res.stream
-  let lhsRefs := lhsRefs.cast <| by
-    apply AIG.LawfulStreamOperator.le_size (f := BVExpr.bitblast)
-  streamProc aig ⟨lhsRefs, rhsRefs⟩
-where
-  streamProc {w : Nat} (aig : AIG BVBit) (input : AIG.BinaryRefStream aig w) : AIG.Entrypoint BVBit :=
-  let ⟨lhsRefs, rhsRefs⟩ := input
+variable [BEq α] [Hashable α] [DecidableEq α]
+
+def mkUlt (aig : AIG α) (pair : AIG.BinaryRefStream aig w) : AIG.Entrypoint α :=
+  let ⟨lhsRefs, rhsRefs⟩ := pair
   let res := BVExpr.bitblast.blastNot aig rhsRefs
   let aig := res.aig
   let rhsRefs := res.stream
@@ -32,10 +23,10 @@ where
   let overflowRef := res.ref
   aig.mkNotCached overflowRef
 
-instance mkUlt_inst {w : Nat} : AIG.LawfulOperator BVBit (AIG.BinaryRefStream · w) mkUlt.streamProc where
+instance {w : Nat} : AIG.LawfulOperator α (AIG.BinaryRefStream · w) mkUlt where
   le_size := by
     intros
-    unfold mkUlt.streamProc
+    unfold mkUlt
     dsimp
     apply AIG.LawfulOperator.le_size_of_le_aig_size (f := AIG.mkNotCached)
     apply AIG.LawfulOperator.le_size_of_le_aig_size (f := BVExpr.bitblast.mkOverflowBit)
@@ -43,7 +34,7 @@ instance mkUlt_inst {w : Nat} : AIG.LawfulOperator BVBit (AIG.BinaryRefStream ·
     apply AIG.LawfulStreamOperator.le_size (f := BVExpr.bitblast.blastNot)
   decl_eq := by
     intros
-    unfold mkUlt.streamProc
+    unfold mkUlt
     dsimp
     rw [AIG.LawfulOperator.decl_eq (f := AIG.mkNotCached)]
     rw [AIG.LawfulOperator.decl_eq (f := BVExpr.bitblast.mkOverflowBit)]
@@ -57,27 +48,6 @@ instance mkUlt_inst {w : Nat} : AIG.LawfulOperator BVBit (AIG.BinaryRefStream ·
     . apply AIG.LawfulOperator.lt_size_of_lt_aig_size (f := BVExpr.bitblast.mkOverflowBit)
       apply AIG.LawfulOperator.lt_size_of_lt_aig_size (f := AIG.mkConstCached)
       apply AIG.LawfulStreamOperator.lt_size_of_lt_aig_size (f := BVExpr.bitblast.blastNot)
-      assumption
-
-instance : AIG.LawfulOperator BVBit (fun _ => ExprPair) mkUlt where
-  le_size := by
-    intros
-    unfold mkUlt
-    dsimp
-    apply AIG.LawfulOperator.le_size_of_le_aig_size (f := mkUlt.streamProc)
-    apply AIG.LawfulStreamOperator.le_size_of_le_aig_size (f := BVExpr.bitblast)
-    apply AIG.LawfulStreamOperator.le_size (f := BVExpr.bitblast)
-  decl_eq := by
-    intros
-    unfold mkUlt
-    dsimp
-    rw [AIG.LawfulOperator.decl_eq (f := mkUlt.streamProc)]
-    rw [AIG.LawfulStreamOperator.decl_eq (f := BVExpr.bitblast)]
-    rw [AIG.LawfulStreamOperator.decl_eq (f := BVExpr.bitblast)]
-    . apply AIG.LawfulStreamOperator.lt_size_of_lt_aig_size (f := BVExpr.bitblast)
-      assumption
-    . apply AIG.LawfulStreamOperator.lt_size_of_lt_aig_size (f := BVExpr.bitblast)
-      apply AIG.LawfulStreamOperator.lt_size_of_lt_aig_size (f := BVExpr.bitblast)
       assumption
 
 end BVPred
