LeanSAT/Reflect/BVExpr/BitBlast/Lemmas/Eq.lean
@@ -1,42 +1,31 @@
 import LeanSAT.Reflect.BVExpr.BitBlast.Lemmas.Basic
-import LeanSAT.Reflect.BVExpr.BitBlast.Lemmas.Expr
 import LeanSAT.Reflect.BVExpr.BitBlast.Impl.Eq
 
 open AIG
 
 namespace BVPred
 
-theorem mkEq_denote_iff_eval_beq (aig : AIG BVBit) (pair : ExprPair) (assign : BVExpr.Assignment)
-    : ⟦mkEq aig pair, assign.toAIGAssignment⟧
-        ↔
-      (pair.lhs.eval assign == pair.rhs.eval assign) := by
-  rw [beq_iff_eq]
+variable [BEq α] [Hashable α] [DecidableEq α]
+
+theorem mkEq_denote_eq_eval_beq (aig : AIG α) (pair : AIG.BinaryRefStream aig w) (assign : α → Bool)
+    (lhs rhs : BitVec w)
+    (hleft : ∀ (idx : Nat) (hidx : idx < w), ⟦aig, pair.lhs.getRef idx hidx, assign⟧ = lhs.getLsb idx)
+    (hright : ∀ (idx : Nat) (hidx : idx < w), ⟦aig, pair.rhs.getRef idx hidx, assign⟧ = rhs.getLsb idx)
+    :  ⟦mkEq aig pair, assign⟧
+         =
+       (lhs == rhs) := by
   unfold mkEq
-  unfold mkEq.streamProc
-  dsimp
+  rw [Bool.eq_iff_iff]
+  simp
   constructor
   . intro h
-    apply BitVec.eq_of_getLsb_eq
-    intro i
-    simp only [RefStream.denote_fold_and, RefStream.denote_zip, RefStream.getRef_cast,
-      denote_mkBEqCached, BVExpr.bitblast_denote_eq_eval_getLsb, beq_iff_eq] at h
-    specialize h i.val i.isLt
-    rw [AIG.LawfulStreamOperator.denote_input_stream (f := BVExpr.bitblast)] at h
-    rw [← h]
-    simp
-  . intro h
-    simp only [RefStream.denote_fold_and, RefStream.denote_zip, RefStream.getRef_cast,
-      denote_mkBEqCached, BVExpr.bitblast_denote_eq_eval_getLsb, beq_iff_eq]
-    intro idx hidx
-    rw [AIG.LawfulStreamOperator.denote_input_stream (f := BVExpr.bitblast)]
+    ext
+    rw [← hleft, ← hright]
+    . simp [h]
+    . omega
+    . omega
+  . intro h idx hidx
+    rw [hleft, hright]
     simp [h]
-
-@[simp]
-theorem mkEq_denote_eq_eval_beq (aig : AIG BVBit) (pair : ExprPair) (assign : BVExpr.Assignment)
-    : ⟦mkEq aig pair, assign.toAIGAssignment⟧
-        =
-      (pair.lhs.eval assign == pair.rhs.eval assign) := by
-  rw [Bool.eq_iff_iff]
-  apply mkEq_denote_iff_eval_beq
 
 end BVPred
